strata-examples/lakefile.lean
@@ -1,0 +1,19 @@
+import Lake
+open Lake DSL
+
+require triptych from ".."
+require StrataDDM from git
+  "https://github.com/strata-org/Strata-DDM" @
+    "247e0512ccd91c0280c1d98401bc7795b6d3a1a4"
+
+package strataExamples
+
+@[default_target]
+lean_lib StrataExamples where
+  globs := #[
+    .one `StrataExamples,
+    .submodules `Inputs,
+    .submodules `Outputs,
+    .submodules `Proofs
+  ]
+  defaultFacets := #[LeanLib.staticFacet]
